Checkpoint intermediate format descriptors

src/InterParse.v
@@ -21,4 +21,93 @@ Module InterParse.
   Import ByteInput.
   Import T.
 
+  (*** Intermediate Complexity Format *)
+
+  (*
+    This format is designed to build on what I've learned from the simple recursive format
+    (SimplParse.v) by adding these features:
+    - Encoding uses tagged key-value pairs which can be read in any order
+    - Uses a single default value for everything / supports optional fields
+    - Does not accept repeated fields
+    - Drops unknown fields without error
+
+    All of these features will be required for protobuf, and will mandate using the RecursiveState 
+    combinator to have access to and change the descriptor during the parsing / serializing process.
+   *)
+
+  Section Desc.
+
+    (* A descriptor is a primitive or a map from w8 to descriptor *)
+    Inductive Desc' : Set := 
+    | D_BOOL
+    | D_INT
+    | D_NEST (fields : gmap w8 Desc').
+
+  (* The "problem" with this definition is that it combines incomplete primitive fields with
+     nested ones, i.e. we can have D_BOOL as a stand-alone descriptor but that can't be serialized
+     without knowing what the field number is.
+   *)
+
+    Inductive Desc : Set := DESC (fs : gmap w8 Field)
+    with
+      Field :=
+    | F_MSG (d : Desc)
+    | F_BOOL
+    | F_INT.
+    
+  (* Instead, use a mutually recursive type so that fields and descriptors (fields with an identifier)
+     are distinct.
+   *)
+
+    Inductive Value : Set := VALUE (vs : gmap w8 Val)
+    with
+      Val :=
+    | V_MSG (v : Value)
+    | V_BOOL (b : bool)
+    | V_INT (b : Z)
+    | V_MISSING.
+
+  (* Define a Value type which matches the structure of the descriptor, with an extra option for
+     missing values, which will also be used as a default value when creating an empty value. *)
+    
+  (* Now in order to use the RecursiveState combinator we need a proposition linking
+     a Value to it's Descriptor. Valid : Desc -> Value -> Prop *)
+
+    Fixpoint Valid (d : Desc) (v : Value) : Prop :=
+      match d, v with
+      | DESC fs, VALUE vs => map_fold (Valid__fold vs) True fs
+      end
+    with Valid__fold (vs : gmap w8 Val) (k : w8) (f : Field) (acc : Prop) : Prop :=
+           match f with
+           | F_BOOL => acc /\ exists b, vs !! k = Some (V_BOOL b)
+           | F_INT => acc /\ exists z, vs !! k = Some (V_INT z)
+           | F_MSG d => acc /\ exists v, vs !! k = Some (V_MSG v) /\ Valid d v
+           end.
+
+    Definition desc1 := DESC (list_to_map [
+                                  (W8 1, F_BOOL);
+                                  (W8 2, F_INT)
+                          ]).
+    Definition val1 := VALUE (list_to_map [
+                                  (W8 1, V_BOOL false);
+                                  (W8 2, V_INT 0)
+                         ]).
+    Lemma test_valid1 : Valid desc1 val1.
+    Proof.
+      simpl.
+      unfold map_fold.
+      unfold gmap_fold. 
+    Abort.
+
+  End Desc.
+
+  Section Parse.
+  End Parse.
+
+  Section Serial.
+  End Serial.
+
+  Section Theorems.
+  End Theorems.
+
 End InterParse.
